ems/STS.v
@@ -20,7 +20,7 @@ Inductive sort: Type :=
 | angelic
 | demonic
 | final (retv: Any.t)
-| vis
+| vis (ev: event)
 .
 
 Record semantics : Type := Semantics_gen {
@@ -32,18 +32,12 @@ Record semantics : Type := Semantics_gen {
   (* wf_vis: forall st0 (VIS: state_sort st0 = vis), exists ev st1, step st0 (Some ev) st1; *)
   (** wf_vis might be completely removed with a new transformation pass *)
   wf_vis: forall
-      st0 ev0 ev1 st1 st2
-      (VIS: state_sort st0 = vis)
+      st0 ev ev0 ev1 st1 st2
+      (VIS: state_sort st0 = vis ev)
       (STEP: step st0 ev0 st1)
       (STEP: step st0 ev1 st2)
     ,
-      (ev0 = ev1 /\ st1 = st2);
-  wf_vis_event: forall
-      st0 ev0 st1
-      (VIS: state_sort st0 = vis)
-      (STEP: step st0 ev0 st1)
-    ,
-      ev0 <> None;
+      (Some ev = ev0 /\ Some ev = ev1 /\ st1 = st2);
   wf_angelic: forall st0 ev st1 (VIS: state_sort st0 = angelic) (STEP: step st0 ev st1), ev = None;
   wf_demonic: forall st0 ev st1 (VIS: state_sort st0 = demonic) (STEP: step st0 ev st1), ev = None;
   wf_final: forall st0 ev st1 r (FIN: state_sort st0 = final r) (STEP: step st0 ev st1), False;
