ems/SimGlobalAlts2Index.v
@@ -36,13 +36,19 @@ Section PROOF.
     ginit. revert_until TOP. gcofix CIH. i.
     revert_until SIM. induction SIM using simg_alt_imp_ind; i.
     { inv TGT. inv SRC. guclo simg_indC_spec. econs 1; eauto. all: refl. }
-    { inv TGT. inv SRC. inv ARG. gstep. econs 2. i. specialize (SIM _ _ EQ).
+    { inv TGT. inv SRC. inv ARG. gstep. econs 2. i. subst. specialize (SIM x_tgt).
       inv SIM. inv REL. clarify. rewrite ! bind_trigger in *.
       inv H0. apply inj_pair2 in H2. eapply equal_f in H2.
       inv H1. apply inj_pair2 in H0. eapply equal_f in H0.
       rewrite H0, H2 in REL0. gfinal. left. eapply CIH. auto.
     }
-    { inv TGT. inv SRC. gstep. econs 10. i. specialize (SIM _ _ EQ).
+    { inv TGT. inv SRC. gstep. econs 3.
+      inv SIM. inv REL. clarify. rewrite ! bind_trigger in *.
+      inv H0. apply inj_pair2 in H2. eapply equal_f in H2.
+      inv H1. apply inj_pair2 in H0. eapply equal_f in H0.
+      rewrite H0, H2 in REL0. gfinal. left. eapply CIH. auto.
+    }
+    { inv TGT. inv SRC. gstep. econs 11. i. specialize (SIM _ _ EQ).
       inv SIM. inv REL. clarify. rewrite ! bind_trigger in *.
       inv H0. apply inj_pair2 in H3. eapply equal_f in H3.
       inv H1. apply inj_pair2 in H4. eapply equal_f in H4.
@@ -51,33 +57,33 @@ Section PROOF.
     { guclo simg_indC_spec. inv SIM.
       - econs; auto. des; eauto.
         guclo simg_indC_spec. inv REL; eauto.
-        + econs; auto. gstep. econs 9. gfinal; left. eauto. all: eapply Ord.S_lt.
-        + des. econs; auto. eexists. gstep. econs 9. gfinal; left. eauto. all: eapply Ord.S_lt.
-        + econs; auto. i. gstep. econs 9. gfinal; left. eauto. all: eapply Ord.S_lt.
+        + econs; auto. gstep. econs 10. gfinal; left. eauto. all: eapply Ord.S_lt.
+        + des. econs; auto. eexists. gstep. econs 10. gfinal; left. eauto. all: eapply Ord.S_lt.
+        + econs; auto. i. gstep. econs 10. gfinal; left. eauto. all: eapply Ord.S_lt.
       - econs; auto. i. specialize (REL x). des; eauto. guclo simg_indC_spec. inv REL; eauto.
-        + econs; auto. gstep. econs 9. gfinal; left. eauto. all: eapply Ord.S_lt.
-        + des. econs; auto. eexists. gstep. econs 9. gfinal; left. eauto. all: eapply Ord.S_lt.
-        + econs; auto. i. gstep. econs 9. gfinal; left. eauto. all: eapply Ord.S_lt.
+        + econs; auto. gstep. econs 10. gfinal; left. eauto. all: eapply Ord.S_lt.
+        + des. econs; auto. eexists. gstep. econs 10. gfinal; left. eauto. all: eapply Ord.S_lt.
+        + econs; auto. i. gstep. econs 10. gfinal; left. eauto. all: eapply Ord.S_lt.
       - destruct REL as [x REL]. econs; auto. exists x. des; eauto.
         guclo simg_indC_spec. inv REL; eauto.
-        + econs; auto. gstep. econs 9. gfinal; left. eauto. all: eapply Ord.S_lt.
-        + des. econs; auto. eexists. gstep. econs 9. gfinal; left. eauto. all: eapply Ord.S_lt.
-        + econs; auto. i. gstep. econs 9. gfinal; left. eauto. all: eapply Ord.S_lt.
+        + econs; auto. gstep. econs 10. gfinal; left. eauto. all: eapply Ord.S_lt.
+        + des. econs; auto. eexists. gstep. econs 10. gfinal; left. eauto. all: eapply Ord.S_lt.
+        + econs; auto. i. gstep. econs 10. gfinal; left. eauto. all: eapply Ord.S_lt.
     }
     { guclo simg_indC_spec. inv SIM.
       - econs; auto. des; eauto. guclo simg_indC_spec. inv REL; eauto.
-        + econs; auto. gstep. econs 9. gfinal; left. eauto. all: eapply Ord.S_lt.
-        + econs; auto. i. gstep. econs 9. gfinal; left. eauto. all: eapply Ord.S_lt.
-        + des. econs; auto. eexists. gstep. econs 9. gfinal; left. eauto. all: eapply Ord.S_lt.
+        + econs; auto. gstep. econs 10. gfinal; left. eauto. all: eapply Ord.S_lt.
+        + econs; auto. i. gstep. econs 10. gfinal; left. eauto. all: eapply Ord.S_lt.
+        + des. econs; auto. eexists. gstep. econs 10. gfinal; left. eauto. all: eapply Ord.S_lt.
       - destruct REL as [x REL]. econs; auto. exists x. des; eauto.
         guclo simg_indC_spec. inv REL; eauto.
-        + econs; auto. gstep. econs 9. gfinal; left. eauto. all: eapply Ord.S_lt.
-        + econs; auto. i. gstep. econs 9. gfinal; left. eauto. all: eapply Ord.S_lt.
-        + des. econs; auto. eexists. gstep. econs 9. gfinal; left. eauto. all: eapply Ord.S_lt.
+        + econs; auto. gstep. econs 10. gfinal; left. eauto. all: eapply Ord.S_lt.
+        + econs; auto. i. gstep. econs 10. gfinal; left. eauto. all: eapply Ord.S_lt.
+        + des. econs; auto. eexists. gstep. econs 10. gfinal; left. eauto. all: eapply Ord.S_lt.
       - econs; auto. i. specialize (REL x). des; eauto. guclo simg_indC_spec. inv REL; eauto.
-        + econs; auto. gstep. econs 9. gfinal; left. eauto. all: eapply Ord.S_lt.
-        + econs; auto. i. gstep. econs 9. gfinal; left. eauto. all: eapply Ord.S_lt.
-        + des. econs; auto. eexists. gstep. econs 9. gfinal; left. eauto. all: eapply Ord.S_lt.
+        + econs; auto. gstep. econs 10. gfinal; left. eauto. all: eapply Ord.S_lt.
+        + econs; auto. i. gstep. econs 10. gfinal; left. eauto. all: eapply Ord.S_lt.
+        + des. econs; auto. eexists. gstep. econs 10. gfinal; left. eauto. all: eapply Ord.S_lt.
     }
     Unshelve. all: exact f_src.
   Qed.
