ems/SimGlobalExplicit2Alts.v
@@ -56,13 +56,14 @@ Section PROOF.
       i.
       econs; eauto. econs; eauto.
       exists (Some (f_tgt1, f_src1)). gfinal. left. eapply CIH; eauto.
-      specialize (SIM0 v0 v eq_refl). pclearbot. eapply SIM0.
+      specialize (SIM0 rv rv eq_refl). pclearbot. eapply SIM0.
     }
     { right. exists (Some (f_tgt, f_src0)). split.
       2:{ econs. econs 2; eauto. }
       gstep. do 2 right. left. pclearbot. exists (rv). splits; [econs; eauto| econs; eauto |].
       i.
-      econs; eauto.
+      econs; eauto. econs; eauto.
+      exists (Some (f_tgt1, f_src1)). gfinal. left. eapply CIH; eauto.
     }
     { pclearbot. right. exists (Some (f_tgt, f_src0)). split.
       2:{ econs. econs 2; eauto. }
@@ -111,11 +112,13 @@ Section PROOF.
       i.
       econs; eauto. econs; eauto.
       exists (Some (f_tgt0, f_src0)). gfinal. left. eapply CIH; eauto.
-      specialize (SIM0 tt↑ tt↑ eq_refl). pclearbot. eapply SIM0.
+      specialize (SIM0 rv rv eq_refl). pclearbot. eapply SIM0.
     }
     { gstep. do 2 right. left. exists (rv). splits; [econs; eauto | econs; eauto |].
       i.
-      econs; eauto.
+      econs; eauto. econs; eauto.
+      exists (Some (f_tgt0, f_src0)). gfinal. left. eapply CIH; eauto.
+      pclearbot. eapply SIM0.
     }
     { destruct SIM0 as [SIM | SIM]; clarify.
       gstep. do 4 right. right. econs 1.
